Towards nice conversions on closed terms

sme/Sme/M/DT/Closed.lean
@@ -22,9 +22,28 @@ def Closed (x : DeepThunk P (α ::: β)) : Prop :=
     (TypeVec.id ::: fun _ => ULift.up Bool.true) <$$> x
   = (TypeVec.id ::: fun _ => ULift.up Bool.false) <$$> x
 
+variable (x : DeepThunk P (α ::: β))
+
 namespace Closed
 
-variable (x : DeepThunk P (α ::: β))
+private theorem snd_fz_h_Closed_of_Closed.helper {y} (h : x = y) z
+    : (HpLuM.dest x).snd .fz z
+    = (HpLuM.dest y).snd .fz (cast (h ▸ rfl) z) := by
+  subst h
+  rfl
+
+theorem snd_fz_h_Closed_of_Closed
+    {x : DeepThunk P (α ::: β)} (h : x.Closed) {h'}
+    : Closed ((HpLuM.dest x).snd Fin2.fz h') := by
+  have := snd_fz_h_Closed_of_Closed.helper _ h (cast (by simp) h')
+  simp only [Nat.succ_eq_add_one, TypeVec.append1_get_fz, comp.B_eq, cast_cast] at this
+  rewrite! [HpLuM.dest_map, MvPFunctor.map_snd] at this
+  simp only [map_fst, cast_eq, TypeVec.comp.get, comp.B_eq, TypeVec.append1_get_fz,
+    TypeVec.appendFun.get_fz, Function.comp_apply] at this
+  rewrite! [HpLuM.dest_map, MvPFunctor.map_snd] at this
+  simp only [map_fst, cast_eq, TypeVec.comp.get, comp.B_eq, TypeVec.append1_get_fz,
+    TypeVec.appendFun.get_fz, Function.comp_apply] at this
+  exact this
 
 private theorem getNext.helper {y} (h : x = y) z
     : (comp.get (HpLuM.dest x)).snd .fz z
@@ -94,19 +113,127 @@ theorem getNext_closed (hC : Closed x) (v : P.B (comp.get (HpLuM.dest x)).fst Fi
       generalize_proofs h'
       exact False.elim (h' _ h)
 
-def change {γ} (x : DeepThunk P (α ::: β)) (h : Closed x) : DeepThunk P (α ::: γ) :=
+def change γ (x : DeepThunk P (α ::: β)) (h : Closed x) : DeepThunk P (α ::: γ) :=
   HpLuM.corec' step ⟨x, h⟩
 where
   step (x : { x : DeepThunk P _ // Closed x}) :=
-    have ⟨x, h⟩ := x
-    letI := comp.get (HpLuM.dest x)
+    letI := comp.get (HpLuM.dest x.1)
     comp.mk ⟨
       this.fst, fun
-      | .fz, i =>
-        comp.mk (DTSum.cont (prj.mk .fz ⟨getNext x h i, getNext_closed x h i⟩))
-      | .fs s, i =>
-        prj.mk (s.add 2) <| show α s from
+      | .fz => fun i => by
+        exact comp.mk (DTSum.cont (prj.mk .fz ⟨getNext x.1 x.2 i, getNext_closed x.1 x.2 i⟩))
+      | .fs s => fun i => prj.mk (s.add 2) <| show α s from
           prj.get (i := s.add 2) <| this.snd (.fs s) i
     ⟩
+
+namespace change
+
+theorem change_step_eq_map
+    {x : DeepThunk P (α ::: β)} (h : Closed x)
+    : (TypeVec.id ::: Subtype.val) <$$> step β ⟨x, h⟩
+    = x.dest := by
+  simp only [Nat.succ_eq_add_one, step]
+  rw [comp.map_mk, map_mk]
+  apply comp.get_ext
+  rw [comp.get_mk]
+  refine Sigma.ext rfl <| heq_of_eq ?_
+  dsimp
+  funext i h
+  rcases i with (_|_)
+  · simp [comp.map_mk, ←getNext_eq]
+  · simp [Fin2.add]
+
+theorem change_step_fz_h_eq
+    {x : DeepThunk P (α ::: β)} (h : Closed x)
+    {h'}
+    : (step β ⟨x, h⟩).snd .fz h'
+    = ⟨
+      x.dest.snd .fz <| cast (by rw [←change_step_eq_map]; rfl) h',
+      snd_fz_h_Closed_of_Closed h
+    ⟩ := by
+  apply Subtype.ext
+  simp only [Nat.succ_eq_add_one, comp.B_eq]
+  rw! [←change_step_eq_map h]
+  rfl
+
+theorem noop {x : DeepThunk P (α ::: β)} (h : Closed x) : change β x h = x := by
+  apply HpLuM.bisim (fun a b => ∃ h, change β b h = a) ⟨h, rfl⟩
+  rintro _ t ⟨h, rfl⟩
+  use t.dest.fst
+  dsimp only [change]
+  rw! [HpLuM.dest_corec']
+  simp only [Nat.succ_eq_add_one, map_fst, map_snd, heq_eq_eq, true_and, comp.B_eq, exists_and_left,
+    ↓existsAndEq]
+  have : t.dest.fst = (@step _ _ _ α β ⟨t, h⟩).fst := by
+    rw [←change_step_eq_map h]
+    simp
+  use (TypeVec.id ::: HpLuM.corec' (step _)) ⊚ (step _ ⟨t, h⟩).snd ⊚ TypeVec.Arrow.mp (by rw [this])
+  simp only [Nat.succ_eq_add_one, TypeVec.comp.get, comp.B_eq, TypeVec.mp.get, Function.comp_apply]
+  refine ⟨⟨this.symm, ?_⟩, ?_⟩
+  · rw [TypeVec.heq_of_mp_mpr rfl (by rw [this])]
+    simp [TypeVec.comp_assoc]
+  rintro (_|i) h
+  <;> simp only [TypeVec.RelLast, TypeVec.append1_get_fs,
+    TypeVec.appendFun.get_fs, TypeVec.id.get, id_eq, TypeVec.appendFun.get_fz]
+  · rw! [change_step_fz_h_eq]
+    simp only [Nat.succ_eq_add_one, comp.B_eq, cast_cast, cast_eq, exists_prop, and_true]
+    apply snd_fz_h_Closed_of_Closed
+    assumption
+  · rw! (castMode := .all) [←change_step_eq_map]
+    rfl
+
+theorem map_step
+    {γ β δ ε h} {f : α ⟹ β}
+    {f' : _ → ε} {g : _ → δ}
+    : (TypeVec.appendFun (TypeVec.appendFun f g ) f') <$$> step γ ⟨x, h⟩
+    = (TypeVec.appendFun (TypeVec.appendFun f id) f') <$$> step δ ⟨x, h⟩ := by
+  apply comp.get_ext
+  simp only [Nat.succ_eq_add_one, step, comp.map_mk, map_mk, comp.get_mk]
+  refine Sigma.ext rfl <| heq_of_eq ?_
+  funext i h
+  rcases i with (_|_)
+  <;> dsimp at h
+  <;> simp only [Fin2.add, Nat.add_eq, Nat.add_zero, TypeVec.comp.get, Function.comp_apply,
+    prj.map_mk, TypeVec.appendFun.get_fs]
+  simp [comp.map_mk]
+
+theorem closed {γ} {x : DeepThunk P (α ::: β)} (h : Closed x) : (change γ x h).Closed := by
+  dsimp [Closed, change]
+  apply HpLuM.bisim_map (fun a b => ∃ x,
+    a = (TypeVec.id ::: fun x ↦ { down := true }) <$$> HpLuM.corec' (step γ) x  ∧
+    b = (TypeVec.id ::: fun x ↦ { down := false }) <$$> HpLuM.corec' (step γ) x)
+    ⟨_, rfl, rfl⟩
+  rintro _ _ ⟨x, rfl, rfl⟩
+  simp only [Nat.succ_eq_add_one, map_fst, HpLuM.dest_map]
+  rw! [MvFunctor.map_map, TypeVec.appendFun_comp', MvFunctor.map_map, TypeVec.appendFun_comp']
+  simp only [TypeVec.id_comp, Function.const_comp]
+  rw! [HpLuM.dest_corec', HpLuM.dest_corec']
+  rw! [MvFunctor.map_map, TypeVec.appendFun_comp', MvFunctor.map_map, TypeVec.appendFun_comp']
+  simp only [TypeVec.comp_id, Function.const_comp]
+  refine ⟨?_, ?_⟩
+  · rw [map_step]
+    symm
+    rw [map_step]
+  intro v
+  rw! (castMode := .all) [HpLuM.dest_map, HpLuM.dest_corec']
+  simp only [eqRec_eq_cast, map_fst, Nat.succ_eq_add_one, map_snd, TypeVec.comp.get,
+    TypeVec.append1_get_fz, TypeVec.appendFun.get_fz, Function.comp_apply, cast_cast]
+  refine ⟨_, rfl, ?_⟩
+  rw! (castMode := .all) [HpLuM.dest_map, HpLuM.dest_corec']
+  simp
+
+theorem contract {γ δ} (x : DeepThunk P (α ::: β)) (h : Closed x) : change δ (change γ x h) (closed h) = (change δ x h) := by
+  dsimp [change]
+  apply HpLuM.bisim_map (fun a b => ∃ x,
+    a = HpLuM.corec' (step δ) ⟨HpLuM.corec' (step γ) x, closed x.2⟩ ∧
+    b = HpLuM.corec' (step δ) x)
+    ⟨_, rfl, rfl⟩
+  rintro _ _ ⟨x, rfl, rfl⟩
+  simp only [Nat.succ_eq_add_one, map_fst, Subtype.exists, HpLuM.dest_corec']
+  rw! [MvFunctor.map_map, TypeVec.appendFun_comp', MvFunctor.map_map, TypeVec.appendFun_comp']
+  dsimp only [TypeVec.comp_id, Function.const_comp]
+  sorry
+
+end change
 
 end Sme.DeepThunk.Closed
